src/Idempotent.v
@@ -193,13 +193,170 @@ Proof.
   apply corr3_from_corr2; eauto.
 Qed.
 
-  Ltac recover_ro_ok := intros;
-    repeat match goal with
-      | [ |- forall_helper _ ] => unfold forall_helper; intros; eexists; intros
-      | [ |- corr3 _ ?pre' _ _ ] => eapply corr3_from_corr2_rx; eauto with prog
-      | [ |- corr3 _ _ _ _ ] => eapply pimpl_ok3; intros
-      | [ |- corr2 _ _ _ ] => step
-      | [ H: crash_xform ?x =p=> ?x |- context [ crash_xform ?x ] ] => rewrite H
-      | [ H: diskIs _ _ |- _ ] => unfold diskIs in *
-      | [ |- pimpl (crash_xform _) _ ] => progress autorewrite with crash_xform
-    end.
+
+
+
+
+
+Lemma corr3_weak_from_corr2_weak_failed:
+  forall (TF TR: Type) pr tr m mr bmr hmr (p: prog TF) (r: prog TR) out
+         (crash: taggedmem -> domainmem -> pred) ppre rpre crashdone_p crashdone_r,
+  exec_recover pr mr empty_mem empty_mem p r out tr
+  -> TF = TR
+  -> possible_crash m mr
+  -> crash bmr hmr m
+  -> (forall bm' hm', crash_xform (crash bm' hm')
+      =p=> ppre crashdone_p crash empty_mem empty_mem)
+  -> (forall bm' hm', crash_xform (crash bm' hm')
+      =p=> rpre crashdone_r crash empty_mem empty_mem)
+  -> {{W pr | ppre W}} p
+  -> {{W pr | rpre W}} r
+  -> out <> RFailed TF TR.
+Proof.
+  intros.
+  generalize dependent m.
+  induction H; intros; try congruence.
+  - edestruct H5; eauto.
+    eapply H3. eapply crash_xform_apply; eauto.
+    repeat (destruct H7; try congruence).
+Qed.
+
+Lemma corr3_weak_from_corr2_weak_finished:
+  forall (TF TR: Type) pr tr m mr bmr hmr (p: prog TF) (r: prog TR) out
+    (crash: taggedmem -> domainmem -> pred) ppre rpre crashdone_p crashdone_r m' bm' hm' v,
+  exec_recover pr mr empty_mem empty_mem p r out tr
+  -> TF = TR
+  -> possible_crash m mr
+  -> crash bmr hmr m
+  -> (forall bm' hm', crash_xform (crash bm' hm')
+      =p=> ppre crashdone_p crash empty_mem empty_mem)
+  -> (forall bm' hm', crash_xform (crash bm' hm')
+      =p=> rpre crashdone_r crash empty_mem empty_mem)
+  -> {{W pr | ppre W}} p
+  -> {{W pr | rpre W}} r
+  -> out = RFinished TR m' bm' hm' v
+  -> crashdone_p m' bm' hm' v /\ trace_secure pr tr.
+Proof.
+  intros.
+  induction H; try congruence.
+  edestruct H5; eauto.
+  - eapply H3. eapply crash_xform_apply; eauto.
+  - split_ors; cleanup; try congruence; split; eauto; congruence.
+Qed.
+
+
+Lemma corr3_weak_from_corr2_weak_recovered:
+  forall (TF TR: Type) mr (p: prog TF) (r: prog TR) out bm hm
+         (crash: taggedmem -> domainmem -> pred) ppre rpre crashdone_p crashdone_r m' bm' hm' v pr tr,
+  exec_recover pr mr bm hm p r out tr
+  -> out = RRecovered TF m' bm' hm' v  
+  -> TF = TR
+  -> forall m bmr hmr,
+    possible_crash m mr
+  -> crash bmr hmr m
+  -> (forall bm' hm', crash_xform (crash bm' hm')
+      =p=> ppre crashdone_p crash bm hm)
+  -> (forall bm' hm', crash_xform (crash bm' hm')
+      =p=> rpre crashdone_r crash empty_mem empty_mem)
+  -> {{W pr | ppre W}} p
+  -> {{W pr | rpre W}} r
+  -> crashdone_r m' bm' hm' v /\ trace_secure pr tr.
+Proof.
+  induction 1; intros; try congruence.
+  - inversion H2; subst; clear H2.
+    edestruct H8; eauto.
+    eapply H6; eapply crash_xform_apply; eauto.
+    split_ors; cleanup; try congruence.
+    inversion H1; subst.
+    edestruct H9; eauto.
+    
+    eapply H7; eapply crash_xform_apply; eauto.
+    split_ors; cleanup; try congruence.
+    split; eauto.
+    apply trace_secure_app; eauto.
+    
+  - inversion H2; subst; clear H2.
+    edestruct H8; eauto.
+    eapply H6; eapply crash_xform_apply; eauto.
+    split_ors; cleanup; try congruence.
+    edestruct IHexec_recover; eauto.
+    split; eauto.
+    apply trace_secure_app; eauto.
+Qed.
+
+Theorem corr3_weak_from_corr2_weak:
+  forall TF TR (p: prog TF) (r: prog TR) pr ppre rpre,
+    {{W pr | ppre W}} p
+  -> {{W pr | rpre W}} r                 
+  -> {{W pr | fun bm hm done crashdone => exists crash,
+        ppre done crash bm hm
+        * [[ forall bm' hm',
+          crash_xform (crash bm' hm')
+          =p=> rpre crashdone crash empty_mem empty_mem ]] W}} p >> r.
+Proof.
+  unfold corr3_weak; intros.
+  destruct H1 as [crash H1].
+  destruct_lift H1.
+  inversion H2; subst.
+  - edestruct H; eauto.
+    split; eauto.
+    split_ors; cleanup; try congruence.
+    left; repeat eexists; eauto.
+  - exfalso.
+    edestruct H; eauto; repeat deex; try congruence.
+    split_ors; cleanup; try congruence.
+  - edestruct H; eauto; repeat deex; try congruence.
+    split_ors; cleanup; try congruence.
+    clear H H1 H2 ppre.    
+    inversion H6; subst.
+    edestruct H0; eauto.
+    eapply H5.
+    eapply crash_xform_apply; eauto.
+    split_ors; cleanup; try congruence.
+    split.
+    right; repeat eexists; eauto.
+    apply trace_secure_app; eauto.
+    
+  - edestruct H; eauto; repeat deex; try congruence.
+    split_ors; cleanup; try congruence.
+    clear H H1 H2 ppre.
+    edestruct corr3_weak_from_corr2_weak_recovered.
+    apply H6.
+    all: eauto.
+
+    split; eauto.
+    right; repeat eexists; eauto.
+    apply trace_secure_app; eauto.
+Qed.
+
+
+Theorem corr3_weak_from_corr2_weak_rx :
+  forall TF TR RF RR pr (p: prog TF) (r:  prog TR)
+         (rxp : TF -> prog RF) (rxr : TR -> prog RR)
+         ppre rpre,
+  {{W pr | ppre W}} Bind p rxp
+  -> {{W pr | rpre W}} Bind r rxr
+  -> {{W pr | fun bm hm done crashdone => exists crash,
+        ppre done crash bm hm        
+        * [[ forall bm' hm',
+          crash_xform (crash bm' hm')
+          =p=> rpre crashdone crash empty_mem empty_mem]] W}} Bind p rxp >> Bind r rxr.
+Proof.
+  intros.
+  apply corr3_weak_from_corr2_weak; eauto.
+Qed.
+
+Ltac recover_ro_ok :=
+  intros;
+  repeat match goal with
+         | [ |- forall_helper _ ] => unfold forall_helper; intros; eexists; intros
+         | [ |- corr3 _ ?pre' _ _ ] => eapply corr3_from_corr2_rx; eauto with prog
+         | [ |- corr3 _ _ _ _ ] => eapply pimpl_ok3; intros
+         | [ |- corr2 _ _ _ ] => step
+         | [ |- corr3_weak _ ?pre' _ _ ] => eapply corr3_weak_from_corr2_weak_rx; eauto with prog
+         | [ |- corr3_weak _ _ _ _ ] => eapply pimpl_ok3_weak; intros
+         | [ |- corr2_weak _ _ _ ] => weakstep
+         | [ H: crash_xform ?x =p=> ?x |- context [ crash_xform ?x ] ] => rewrite H
+         | [ H: diskIs _ _ |- _ ] => unfold diskIs in *
+         | [ |- pimpl (crash_xform _) _ ] => progress autorewrite with crash_xform
+         end.
